src/canonize/pterm.lean
@@ -1,11 +1,39 @@
 import .nterm
 
+namespace list
+
+theorem filter_perm {α} {p : α → Prop} [decidable_pred p] {l : list α} :
+  l ~ l.filter p ++ l.filter (not ∘ p) :=
+begin
+  induction l with x xs ih,
+  { simp },
+  { by_cases hx : p x,
+    { simp [filter, hx, perm.skip, ih] },
+    { calc
+      x::xs ~ x::(filter p xs ++ filter (not ∘ p) xs) : perm.skip _ ih
+      ... ~ filter p xs ++ x::filter (not ∘ p) xs : perm.symm perm_middle
+      ... ~ filter p (x::xs) ++ filter (not ∘ p) (x::xs) : by simp [hx] }}
+end
+
+theorem prod_ones {α} [monoid α] {l : list α} :
+  (∀ x : α, x ∈ l → x = 1) → l.prod = 1 :=
+begin
+  intro h,
+  induction l with x xs ih,
+  { refl },
+  { have h1 : x = 1, by { apply h, simp },
+    have h2 : prod xs = 1, by { apply ih, intros _ hx, apply h, simp [hx] },
+    simp [h1, h2] }
+end
+
+end list
+
 namespace polya
 
 open nterm
 
 variables {α : Type} [discrete_field α]
-variables {γ : Type} [coeff γ]
+variables {γ : Type} [const_space γ]
 variables [morph γ α] {ρ : dict α}
 
 --@[derive decidable_eq]
@@ -15,70 +43,29 @@ structure xterm : Type :=
 
 namespace xterm
 
---TODO: unable to derive decidable_eq
-instance decidable_eq : decidable_eq (@xterm γ _) := sorry
-
 def le (x y : @xterm γ _) : Prop := x.term ≤ y.term
 
 instance : has_le (@xterm γ _) := ⟨le⟩
 instance : decidable_rel (@xterm.le γ _) := by delta xterm.le; apply_instance
 
-def mul (x : @xterm γ _) (n : znum) : @xterm γ _ :=
-⟨x.term, x.exp * n⟩
-
-def of_nterm (x : @nterm γ _) : @xterm γ _ :=
-⟨x, 1⟩
-
 def to_nterm (x : @xterm γ _) : @nterm γ _ :=
-if x.exp = 0 then 1
+if x.exp = 0 then x.term / x.term
 else if x.exp = 1 then x.term
 else x.term ^ x.exp
 
 def eval (ρ : dict α) (x : @xterm γ _) : α :=
-x.term.eval ρ ^ (x.exp : ℤ)
+let a := nterm.eval ρ x.term in
+if a = 0 then 0 else a ^ (x.exp : ℤ)
 
-theorem eval_def {x : @nterm γ _} {n : znum} :
-  eval ρ ⟨x, n⟩ = x.eval ρ ^ (n : ℤ) :=
-rfl
-
-theorem eval_add' {x : @nterm γ _} {n m : znum} :
-  nterm.eval ρ x ≠ 0 → xterm.eval ρ ⟨x, n + m⟩ = xterm.eval ρ ⟨x, n⟩ * xterm.eval ρ ⟨x, m⟩ :=
+def eval_to_nterm {x : @xterm γ _} :
+ nterm.eval ρ x.to_nterm = xterm.eval ρ x :=
 begin
-  intro hx,
-  simp [xterm.eval, fpow_add hx]
-end
-
-theorem eval_add (x : @nterm γ _) (n m : znum) :
-  n + m ≠ 0 → xterm.eval ρ ⟨x, n + m⟩ = xterm.eval ρ ⟨x, n⟩ * xterm.eval ρ ⟨x, m⟩ :=
-begin
-  intro h1,
-  have h2 : n ≠ 0 ∨ m ≠ 0, by { sorry },
-  by_cases hx : nterm.eval ρ x = 0,
-  { simp only [eval], rw hx,
-    apply eq.trans,
-    { apply zero_fpow,
-      rw ← znum.cast_zero,
-      exact_mod_cast h1 },
-    { rw zero_eq_mul,
-      cases h2,
-      { left, apply zero_fpow,
-        rw ← znum.cast_zero,
-        exact_mod_cast h2 },
-      { right, apply zero_fpow,
-        rw ← znum.cast_zero,
-        exact_mod_cast h2 }}},
-  { simp [eval, fpow_add, hx] }
-end
-
-theorem eval_to_nterm (x : @xterm γ _) :
-  x.to_nterm.eval ρ = x.eval ρ :=
-begin
-  unfold to_nterm, unfold eval,
-  by_cases h1 : x.exp = 0,
-  { simp [h1] },
-  { by_cases h2 : x.exp = 1,
-    { simp [h2] },
-    { simp [h1, h2] }}
+  by_cases hx : nterm.eval ρ x.term = 0;
+  { by_cases h1 : x.exp = 0,
+    { simp [hx, h1, nterm.eval, xterm.eval, to_nterm] },
+    { have : (x.exp : ℤ) ≠ 0, by {rw ← znum.cast_zero, exact_mod_cast h1 },
+      by_cases h2 : x.exp = 1;
+      simp [hx, h1, h2, nterm.eval, xterm.eval, to_nterm, zero_fpow, this] }}
 end
 
 theorem eval_to_nterm' :
@@ -88,207 +75,166 @@ begin
   simp [eval_to_nterm]
 end
 
-theorem eval_mul {x : @xterm γ _} {n : znum} :
-  (x.mul n).eval ρ = x.eval ρ ^ (n : ℤ) :=
-by simp [mul, eval, fpow_mul] 
+theorem eval_def {x : @nterm γ _} {n : znum} :
+  xterm.eval ρ ⟨x, n⟩ =
+    if nterm.eval ρ x = 0 then 0
+    else nterm.eval ρ x ^ (n : ℤ) :=
+rfl
+
+theorem eval_add {x : @nterm γ _} {n m : znum} :
+  xterm.eval ρ ⟨x, n + m⟩ = xterm.eval ρ ⟨x, n⟩ * xterm.eval ρ ⟨x, m⟩ :=
+begin
+  by_cases hx : nterm.eval ρ x = 0;
+  simp [xterm.eval, fpow_add, hx]
+end
 
 end xterm
 
 structure pterm : Type :=
 (terms : list (@xterm γ _))
+(coeff : γ)
 
 namespace pterm
 
-def append (P1 P2 : @pterm γ _) : @pterm γ _ :=
-⟨P1.terms ++ P2.terms⟩
+instance : has_zero (@pterm γ _) :=
+⟨{ terms := [],
+   coeff := 0,
+}⟩
 
-instance : has_append (@pterm γ _) := ⟨append⟩
-
-theorem append_terms (P1 P2 : @pterm γ _) :
-  (P1 ++ P2).terms = P1.terms ++ P2.terms := rfl
-
-def mul (P : @pterm γ _) (n : znum) : @pterm γ _ :=
-if n = 0 then ⟨[]⟩
-else if n = 1 then P
-else ⟨P.terms.map (λ x, x.mul n)⟩
+instance : has_one (@pterm γ _) :=
+⟨{ terms := [],
+   coeff := 1,
+}⟩
 
 def eval (ρ : dict α) (P : @pterm γ _) : α :=
-list.prod (P.terms.map (xterm.eval ρ))
+list.prod (P.terms.map (xterm.eval ρ)) * morph.f _ P.coeff
 
-
-theorem eval_mul (P : @pterm γ _) (n : znum) :
-(P.mul n).eval ρ = P.eval ρ ^ (n : ℤ) :=
-begin
-  by_cases h : n = 0 ∨ n = 1,
-  { cases h with h h,
-    { simp [h, mul, eval] },
-    { simp [h, mul, eval] }},
-  { have h0 : ¬ n = 0, by { intro h0, apply h, left, exact h0 },
-    have h1 : ¬ n = 1, by { intro h1, apply h, right, exact h1 },
-    cases P with terms,
-    simp [h0, h1, mul, eval], 
-    induction terms with x xs ih,
-    { simp },
-    { simp [ih, mul_fpow, xterm.eval_mul] }
+def mul (P1 P2 : @pterm γ _) : @pterm γ _ :=
+if P1.coeff = 0 ∨ P2.coeff = 0 then
+  { terms := [],
+    coeff := 0,
   }
+else
+  { terms := P1.terms ++ P2.terms,
+    coeff := P1.coeff * P2.coeff,
+  }
+
+def pow (P : @pterm γ _) (m : znum) : @pterm γ _ :=
+if m = 0 then 1
+else
+  { terms := P.terms.map (λ ⟨x, n⟩, ⟨x, n + m⟩),
+    coeff := P.coeff ^ (m : ℤ),
+  }
+
+instance : has_mul (@pterm γ _) := ⟨mul⟩
+instance : has_pow (@pterm γ _) znum := ⟨pow⟩
+
+theorem mul_terms {P Q : @pterm γ _} :
+  P.coeff ≠ 0 ∧ Q.coeff ≠ 0 →
+  (P * Q).terms = P.terms ++ Q.terms :=
+begin
+  intro h,
+  simp [has_mul.mul, mul, h] 
 end
 
-theorem eval_append (P1 P2 : @pterm γ _) :
-  (P1 ++ P2).eval ρ = P1.eval ρ * P2.eval ρ :=
+theorem mul_terms' {P Q : @pterm γ _} :
+  P.coeff = 0 ∨ Q.coeff = 0 →
+  (P * Q).terms = [] :=
 begin
-  unfold eval,
-  simp only [append_terms],
-  rw [list.map_append],
-  apply list.prod_append 
+  intro h,
+  simp [has_mul.mul, mul, h]
+end
+
+theorem mul_coeff {P Q : @pterm γ _} :
+  (P * Q).coeff = P.coeff * Q.coeff :=
+begin
+  by_cases h : P.coeff = 0 ∨ Q.coeff = 0,
+  { apply eq.trans,
+    { show (P * Q).coeff = 0, simp [has_mul.mul, mul, h] },
+    { simp [h] }},
+  { simp [has_mul.mul, mul, h] }
+end
+
+theorem eval_mul {P Q : @pterm γ _} :
+  pterm.eval ρ (P * Q) = pterm.eval ρ P * pterm.eval ρ Q :=
+begin
+  unfold pterm.eval, rw mul_coeff,
+  by_cases h0 : P.coeff = 0 ∨ Q.coeff = 0,
+  { cases h0; simp [h0, morph.morph0] },
+  { have : P.coeff ≠ 0 ∧ Q.coeff ≠ 0,
+    from (decidable.not_or_iff_and_not _ _).mp h0,
+    rw [mul_terms this, list.map_append, list.prod_append, morph.morph_mul],
+    ring }
 end
 
 def to_nterm (P : @pterm γ _) : @nterm γ _ :=
-prod (P.terms.map (xterm.to_nterm))
+prod (P.terms.map (xterm.to_nterm)) * P.coeff
 
 theorem eval_to_nterm {P : @pterm γ _} :
-  P.eval ρ = P.to_nterm.eval ρ :=
+  pterm.eval ρ P = nterm.eval ρ P.to_nterm :=
 begin
-  cases P with terms,
-  unfold to_nterm, unfold eval,
+  cases P with terms coeff ts,
+  suffices : list.prod (list.map (xterm.eval ρ) terms) * morph.f α coeff =
+    nterm.eval ρ (prod (list.map xterm.to_nterm terms)) * morph.f α coeff,
+  by simp [to_nterm, pterm.eval, this],
   rw [eval_prod, list.map_map],
   rw xterm.eval_to_nterm'
 end
 
-structure reduce_cache : Type :=
-(t : @xterm γ _)
-(ts : list (@xterm γ _))
-(hyps : list (@nterm γ _))
+def filter (P : @pterm γ _) : @pterm γ _ :=
+{ terms := P.terms.filter (λ x, x.exp ≠ 0),
+  coeff := P.coeff
+}
 
-def reduce_cache.eval (ρ : dict α) (pi : @reduce_cache γ _) : α :=
-if nterm.eval ρ pi.t.term = 0 then 0
-else xterm.eval ρ pi.t * pterm.eval ρ ⟨pi.ts⟩
+def filter_hyps (P : @pterm γ _) : list (@nterm γ _) :=
+list.map xterm.term (P.terms.filter (λ x, x.exp = 0))
 
-def reduce_aux : @reduce_cache γ _ → @xterm γ _ → @reduce_cache γ _
-| ⟨⟨x, n⟩, ts, hyps⟩ ⟨y, m⟩ :=
-  if m = 0 then
-    ⟨⟨x, n⟩, ts, hyps⟩
-  else if x = y then
-    ⟨⟨x, n + m⟩, ts, hyps⟩
-  else if n = 0 then
-    ⟨⟨y, m⟩, ts, x::hyps⟩
-  else
-    ⟨⟨y, m⟩, ⟨x, n⟩::ts, hyps⟩
-
-def reduce_ih (ρ : dict α) (c : α) (pi : @reduce_cache γ _) : Prop :=
-  (∀ h ∈ pi.hyps, nterm.eval ρ h ≠ 0) → pi.eval ρ = c
-
-theorem eval_reduce_aux (c : α) (y : @xterm γ _)
-  (pi : @reduce_cache γ _)
-  (ih : reduce_ih ρ c pi) :
-  reduce_ih ρ (xterm.eval ρ y * c) (reduce_aux pi y) :=
+private lemma lemma_eval_filter {x : @xterm γ _} :
+  x.exp = 0 ∧ nterm.eval ρ x.term ≠ 0 →
+  xterm.eval ρ x = 1 :=
 begin
-  cases pi with x xs ts,
   cases x with x n,
-  cases y with y m,
-  intro H,
-  have H' : ∀ t ∈ ts, nterm.eval ρ t ≠ 0,
-  by {
-    by_cases h1 : m = 0,
-    { simp [reduce_aux, h1] at H, apply H },
-    { by_cases h2 : x = y,
-      { simp [reduce_aux, h1, h2] at H, apply H },
-      { by_cases h3 : n = 0,
-        { simp [reduce_aux, h1, h2, h3] at H, apply H.right },
-        { simp [reduce_aux, h1, h2, h3] at H, apply H }}}},
-  have ih' := ih H',
-  have hc : nterm.eval ρ x = 0 → c = 0,
-  by { intro hx, rw ← ih H', simp [reduce_cache.eval, hx] },
-  
-  by_cases h1 : m = 0,
-  { simp [reduce_aux, xterm.eval, h1, ih H'] },
-  by_cases hy : nterm.eval ρ y = 0,
-  { have : (0 : α) ^ (m : ℤ) = 0,
-    by { apply zero_fpow, rw ← znum.cast_zero, exact_mod_cast h1 },
-    by_cases h2 : x = y; by_cases h3 : n = 0;
-    simp [reduce_aux, reduce_cache.eval, xterm.eval, h1, h2, h3, hy, this] },
-  by_cases h2 : x = y,
-  { have hx : nterm.eval ρ x ≠ 0, by rw h2; exact hy,
-    suffices : xterm.eval ρ ⟨y, n + m⟩ * pterm.eval ρ ⟨xs⟩ = xterm.eval ρ ⟨y, m⟩ * c,
-    by simp [reduce_aux, reduce_cache.eval, h1, h2, hy, this],
-    calc
-    xterm.eval ρ ⟨y, n + m⟩ * pterm.eval ρ ⟨xs⟩
-        = xterm.eval ρ ⟨y, n⟩ * xterm.eval ρ ⟨y, m⟩ * pterm.eval ρ ⟨xs⟩ : by rw xterm.eval_add' hy
-    ... = xterm.eval ρ ⟨y, m⟩ * (xterm.eval ρ ⟨y, n⟩ * pterm.eval ρ ⟨xs⟩) : by ring
-    ... = xterm.eval ρ ⟨y, m⟩ * c : by { rw ← ih H', rw ← h2, simp [reduce_cache.eval, hx] }
-  },
-  by_cases h3 : n = 0,
-  { have h3' : (n : ℤ) = 0, by { rw ← znum.cast_zero, exact_mod_cast h3 },
-    suffices : xterm.eval ρ ⟨y, m⟩ * pterm.eval ρ ⟨xs⟩ = xterm.eval ρ ⟨y, m⟩ * c,
-    by simp [reduce_aux, reduce_cache.eval, h1, h2, h3, hy, this],
-    have hx : nterm.eval ρ x ≠ 0,
-    by { apply H, simp [reduce_aux, h1, h2, h3] },
-    simp [reduce_cache.eval, xterm.eval, hx, h3] at ih',
-    rw ih' },
-  have h3' : (n : ℤ) ≠ 0, by { rw ← znum.cast_zero, exact_mod_cast h3 },
-  by_cases hx : nterm.eval ρ x = 0,
-  { simp [reduce_aux, reduce_cache.eval, xterm.eval, pterm.eval, h1, h2, h3, hy, hx, hc, zero_fpow, h3'] },
-  simp [reduce_cache.eval, xterm.eval, hx] at ih',
-  rw ← ih',
-  simp [reduce_aux, h1, h2, h3, reduce_cache.eval, hx, xterm.eval, hy, pterm.eval]
-
+  simp only [],
+  intro h, cases h with hn hx,
+  simp [xterm.eval, hn, hx]
 end
 
-def reduce (P : @pterm γ _) : list (@nterm γ _) × @pterm γ _ :=
-sorry
-
-theorem eval_reduce {P : @pterm γ _} :
-  (∀ t ∈ P.reduce.fst, nterm.eval ρ t ≠ 0) → P.eval ρ = P.reduce.snd.eval ρ :=
-by sorry
-
-def sort (P : @pterm γ _) : @pterm γ _ :=
-⟨P.terms.merge_sort (≤)⟩
-
-theorem eval_sort {P : @pterm γ _} :
-  P.eval ρ = P.sort.eval ρ :=
+theorem eval_filter {P : @pterm γ _} :
+  (0 : α) ∉ P.filter_hyps.map (nterm.eval ρ) →
+  pterm.eval ρ P = pterm.eval ρ P.filter :=
 begin
-  unfold eval, unfold sort,
-  apply list.prod_eq_of_perm,
-  apply list.perm_map,
-  apply list.perm.symm,
-  apply list.perm_merge_sort
+  intro H,
+  have H1 : ∀ x : xterm, x ∈ P.terms → x.exp = 0 → nterm.eval ρ (x.term) ≠ 0,
+  by simpa [filter_hyps] using H,
+  have H2 : ∀ x : xterm, x ∈ P.terms.filter (λ x, x.exp = 0) → nterm.eval ρ (x.term) ≠ 0,
+  by { intros x hx, have : x ∈ P.terms ∧ x.exp = 0, from list.mem_filter.mp hx,
+       cases this, apply H1; assumption },
+
+  have : P.terms ~ P.terms.filter (λ x, x.exp = 0) ++ P.terms.filter (λ x, x.exp ≠ 0),
+  from list.filter_perm,
+
+  unfold pterm.eval,
+  rw list.prod_eq_of_perm (list.perm_map _ this),
+  rw [list.map_append, list.prod_append],
+
+  have : ∀ x ∈ P.terms.filter (λ x, x.exp = 0), xterm.eval ρ x = 1,
+  by {
+    intros x hx,
+    apply lemma_eval_filter,
+    split,
+    { exact (list.mem_filter.mp hx).right },
+    { apply H2, exact hx }},
+
+  have : ∀ a ∈ (list.map (xterm.eval ρ) (P.terms.filter (λ x, x.exp = 0))), a = 1,
+  by { intros a ha, rw list.mem_map at ha,
+    cases ha with x hx,
+    cases hx with hx ha,
+    rw ← ha, apply this,
+    assumption },
+
+  simp [filter, list.prod_ones this]
 end
 
 end pterm
-
-namespace nterm
-
-def to_pterm : @nterm γ _ → @pterm γ _
-| (mul x y) := x.to_pterm ++ y.to_pterm
-| (pow x n) := x.to_pterm.mul n
-| x := ⟨[⟨x, 1⟩]⟩
-
-theorem eval_to_pterm {x : @nterm γ _} :
-  nterm.eval ρ x = pterm.eval ρ x.to_pterm :=
-begin
-  induction x with i c x y ihx ihy x y ihx ihy x n ihx,
-  { simp [to_pterm, nterm.eval, pterm.eval, xterm.eval] },
-  { simp [to_pterm, nterm.eval, pterm.eval, xterm.eval] },
-  { simp [to_pterm, nterm.eval, pterm.eval, xterm.eval] },
-  { unfold to_pterm, unfold eval,
-    rw [pterm.eval_append, ihx, ihy] },
-  { unfold to_pterm, unfold eval,
-    rw [pterm.eval_mul, ihx] }
-
-end
-
-def norm (x : @nterm γ _) : list (@nterm γ _) × @nterm γ _ :=
-let pi := x.to_pterm.sort.reduce in
-(pi.fst, pi.snd.to_nterm)
-
-theorem correctness {x : @nterm γ _} :
-  (∀ t ∈ x.norm.fst, nterm.eval ρ t ≠ 0) → x.eval ρ = x.norm.snd.eval ρ :=
-assume h,
-calc
-  x.eval ρ = pterm.eval ρ x.to_pterm                 : eval_to_pterm
-       ... = pterm.eval ρ x.to_pterm.sort            : pterm.eval_sort
-       ... = pterm.eval ρ x.to_pterm.sort.reduce.snd : pterm.eval_reduce h
-       ... = nterm.eval ρ x.norm.snd                 : pterm.eval_to_nterm
-
-end nterm
 
 end polya
